WasmInputs/newYear.wat
@@ -1,6 +1,6 @@
 (module
-  (func $main (result f32)
-    (f32.const 9.0)
-    (f32.sqrt)
+  (func $t1 (result f32)
+    (f32.const 3.7)
+    (f32.floor)
   )
 )
