obj/Debug/net9.0/BoogieAST/Debug/BoogieAST.AssemblyInfo.cs
@@ -13,7 +13,7 @@ using System.Reflection;
 [assembly: System.Reflection.AssemblyCompanyAttribute("BoogieAST")]
 [assembly: System.Reflection.AssemblyConfigurationAttribute("Debug")]
 [assembly: System.Reflection.AssemblyFileVersionAttribute("0.1.1.0")]
-[assembly: System.Reflection.AssemblyInformationalVersionAttribute("0.1.1-alpha+ded6dad5d271a0d9d913844d67f4bcfb9cb59a7c")]
+[assembly: System.Reflection.AssemblyInformationalVersionAttribute("0.1.1-alpha+cf965c26bc903f145d5e04c2f0b2c800409299f5")]
 [assembly: System.Reflection.AssemblyProductAttribute("BoogieAST")]
 [assembly: System.Reflection.AssemblyTitleAttribute("BoogieAST")]
 [assembly: System.Reflection.AssemblyVersionAttribute("0.1.1.0")]
